\documentclass[a4paper, 11pt]{article}
\usepackage{fullpage}
\usepackage{amsmath}
\usepackage{amssymb}
\usepackage{mathtools}
\usepackage{enumitem}
\usepackage{multicol}
\usepackage[margin=.25cm]{geometry}
\usepackage{graphicx}
\usepackage{listings}
\usepackage{seqsplit}
\usepackage{tikz}
\usepackage{mathabx}
\usepackage{dashrule}

\newcommand\encircle[1]{%
	\tikz[baseline=(X.base)] 
	\node (X) [draw, shape=circle, inner sep=0] {\strut #1};}

\begin{document}
\pagestyle{empty}
	% Fourier Series
	\begin{multicols}{2}
		\noindent \fbox{\textbf{CTFS}}
		
		\begin{flalign*}
			a_k &= \frac{1}{T}\int_{<T>}^{}x(t)e^{-jk\omega_ot}dt &\\
			x(t) &= \sum_{k=-\infty}^{\infty}a_ke^{j\omega_ot} &
		\end{flalign*}
		
		\noindent FINISH
		
		\noindent \hrulefill
		\columnbreak
		
		\noindent \fbox{\textbf{DTFS}}
		\begin{flalign*}
			a_m &= \frac{1}{N}\sum_{n \in <N>}x[n]e^{\-jm\omega_on} &\\
			x[n] &= \sum_{m \in <N>}a_me^{jm\omega_on} &
		\end{flalign*}
		
		\noindent FINISH
		
		\noindent \hrulefill
	\end{multicols}
	
	% Fourier Transforms
	\begin{multicols}{2}
		\noindent \fbox{\textbf{CTFT}}
		
		\begin{flalign*}
			X(j\omega) &= \int_{-\infty}^{\infty}x(t)e^{-j\omega t}dt & \\
			x(t) &= \frac{1}{2\pi}\int_{-\infty}^{\infty}X(j\omega)e^{j\omega t}d\omega & \\
			X(j\omega_1, j\omega_2) &= \int_{-\infty}^{\infty}\int_{-\infty}^{\infty}x(t_1, t_2)e^{-j\omega_1t_1}e^{-j\omega_2t_2}dt_1dt_2 & \\
			x(t_1, t_2) &= \frac{1}{(2\pi)^2}\int_{-\infty}^{\infty}\int_{-\infty}^{\infty}X(j\omega_1, j\omega_2)e^{j\omega_1t_1}e^{j\omega_2t_2}d\omega_1d\omega_2 &
		\end{flalign*}
		\dotfill
		\begin{enumerate}
			\item Linear\\
				$\alpha x(t) + \beta y(t) \longleftrightarrow \alpha X(j\omega) + \beta Y(j\omega)$
			\item Time Shift\\
				$x(t-\tau) \longleftrightarrow X(j\omega)e^{-j\omega\tau}$
			\item Conjugation\\
				$x^*(t) \longleftrightarrow X^*(-j\omega)$
			\item Conjugate Symmetry\\
				$x(t) \in \mathbb{R} \Longrightarrow x(t) = x^*(t)$\\
				$\cdots \Longrightarrow X(j\omega) = X^*(-j\omega)$
			\item Differentiation\\
				$\frac{dx}{dt} \longleftrightarrow j\omega X(j\omega)$
			\item Integration\\
				$\int_{-\infty}^{t}x(\tau)d\tau \longleftrightarrow \frac{1}{j\omega}X(j\omega) + \pi X(0)\delta (\omega)$
			\item Time/Frequency Scaling\\
				$x(\alpha t) \longleftrightarrow \frac{1}{|\alpha |}X(\frac{j\omega}{\alpha})$
			\item Convolution\\
				$x(t) \convolution y(t) \longleftrightarrow X(j\omega)Y(j\omega)$
			\item Differentiation 2\\
				$-jtx(t) \longleftrightarrow \frac{dX}{d\omega}$
			\item Frequency Shift\\
				$e^{j\omega_ot}x(t) \longleftrightarrow X(j(\omega - \omega_o))$
			\item Multiplication\\
				$x(t)y(t) \longleftrightarrow \frac{1}{2\pi}X(j\omega) * Y(j\omega)$
			\item Separability (Fubini's Theorem?)\\
				$X(j\omega_1, j\omega_2) = X(j\omega_1)X(j\omega_2)$
		\end{enumerate}
		FINISH
		
		\columnbreak
		\noindent \fbox{\textbf{DTFT}} (many repeats from CTFT)
		\begin{flalign*}
			X(e^{j\omega}) &= \sum_{n=\infty}^{\infty}x[n]e^{-j\omega n} &\\
			x[n] &= \frac{1}{2\pi}\int_{<2\pi>}X(e^{j\omega})e^{j\omega n}d\omega
		\end{flalign*}
		\dotfill
		\begin{flalign*}
			\text{Given} &\sum_{k=0}^{N}a_ky[n-k] = \sum_{k=0}^{M}b_kx[n-k]\\
			H(e^{j\omega}) &= \frac{\sum_{k=0}^{M}b_ke^{-j\omega k}}{\sum_{k=0}^{N}a_ke^{-j\omega k}}
		\end{flalign*}
		\dotfill
		\begin{enumerate}
			\item Time Reversal\\
				$x[-n] \longleftrightarrow X(e^{-j\omega})$
			\item Conjugation/Even Symmetry\\
				$x[n] \in \mathbb{R} \Longrightarrow X(e^{j\omega} = X^*(e^{-j\omega}))$\\
				$\cdots \land x[n] = x[-n] \Longrightarrow X(e^{j\omega}) \in \mathbb{R}$
			\item Differencing\\
				$x[n] - x[n-1] \longleftrightarrow X(e^{j\omega})\cdot (1 - e^{-j\omega})$
			\item Accumulation\\
				$\sum_{m=-\infty}^{n}x[m] \longleftrightarrow \frac{1}{1 - e^{-j\omega}}X(e^{j\omega}) + \pi X(e^{0})\sum_{l}\delta(\omega - kl)$
			\item Differentiation\\
				$nx[n] \longleftrightarrow j\frac{dX}{d\omega}$
			\item Parseval's\\
				$\sum_{n=-\infty}^{\infty}|x[n]|^2 = \frac{1}{2\pi}\int_{<2\pi>}|X(e^{j\omega})|^2d\omega$
			\item Multiplication\\
				$x[n]y[n] \longleftrightarrow X(e^{j\omega})\ \ocoasterisk \ Y(e^{j\omega})$\\
				$\cdots \longleftrightarrow \frac{1}{2\pi}\int_{<2\pi>}X(e^{j\theta})Y(e^{j(\omega - \theta)})d\theta$
		\end{enumerate}
		FINISH
	\end{multicols}
	\noindent \fbox{\textbf{DFT}} (finite length sequences)
	\begin{flalign*}
		X[k] &= \sum_{n=0}^{N-1}x[n]e^{-j(\frac{2\pi}{N})kn} k \in [0, N-1]\longrightarrow X[k_1, k_2] = \sum_{n_1=0}^{N_1-1}\sum_{n_2=0}^{N_2-1}x[n_1,n_2]e^{-j(\frac{2\pi}{N_1})k_1n_1}e^{-j(\frac{2\pi}{N_2})k_2n_2}&\\
			&= Na_k\\
		x[n] &= \frac{1}{N}\sum_{k=0}^{N-1}X[k]e^{j(\frac{2\pi}{N})kn} \longrightarrow x[n_1, n_2] = \frac{1}{N_1N_2}\sum_{k_1=0}^{N_1-1}\sum{k_2=0}^{N_2-1}X[k_1, k_2]e^{j(\frac{2\pi}{N_1})k_1n_1}e^{j(\frac{2\pi}{N_2})k_2n_2}
	\end{flalign*}
	\dotfill
	\begin{enumerate}
		\item Conjugate Symmetry\\
			$x[n] \in \mathbb{R} \Longrightarrow X[k] = X^*[N-k] \Longrightarrow X[\frac{N}{2}] \in \mathbb{R}$
	\end{enumerate}
	\hrulefill
	\begin{multicols}{2}
		\noindent \fbox{\textbf{Laplace}}
		\begin{flalign*}
			X(s) &= \int_{-\infty}^{\infty}x(t)e^{-st}dt &\\
			asdf
		\end{flalign*}
		\columnbreak
		asdf
	\end{multicols}
\end{document}